src/SignedBigInteger/LLVM_CodeGen_Signed.thy
@@ -2,6 +2,37 @@ theory LLVM_CodeGen_Signed
   imports Arithmetics "../LLVM_CodeGen" LLVM_CodeGen_Auxiliary UnsignedArithmetics
 begin
 
+section "Comparisons"
+
+sepref_register "op_neq :: bool \<Rightarrow> _"
+sepref_def signed_big_int_eq_impl is "uncurry signed_big_int_eq"
+  :: \<open>sbi_aux_assn\<^sup>k *\<^sub>a sbi_aux_assn\<^sup>k \<rightarrow>\<^sub>a bool1_assn\<close>
+  unfolding signed_big_int_eq_def
+  apply (annot_snat_const size_t)
+  by sepref
+
+sepref_def signed_big_int_neq_impl is "uncurry signed_big_int_neq"
+  :: "sbi_aux_assn\<^sup>k *\<^sub>a sbi_aux_assn\<^sup>k \<rightarrow>\<^sub>a bool1_assn"
+  unfolding signed_big_int_neq_def
+  by sepref
+
+section "Constants"
+
+sepref_def signed_big_int0_impl is "uncurry0 (RETURN signed_big_int0)"
+  :: "unit_assn\<^sup>k \<rightarrow>\<^sub>a sbi_aux_assn"
+  unfolding signed_big_int0_def
+  apply (rewrite al_fold_custom_empty[where 'l=size_t])
+  by sepref
+
+lemma signed_big_int1_alt:
+  "signed_big_int1 = (op_al_empty TYPE(size_t) @ [1], False)"
+  by (simp add: signed_big_int1_def)
+
+sepref_def signed_big_int1_impl is "uncurry0 (RETURN signed_big_int1)"
+  :: "unit_assn\<^sup>k \<rightarrow>\<^sub>a sbi_aux_assn"
+  unfolding signed_big_int1_alt
+  by sepref
+
 section "Unsigned Arithmetics"
 
 sepref_def signed_big_int_add_loop_impl is "uncurry2 signed_big_int_add_loop"
@@ -45,16 +76,17 @@ sepref_def signed_big_int_add_\<sigma>_eq_impl is "uncurry signed_big_int_add_\<
   :: "sbi_aux_assn\<^sup>k *\<^sub>a sbi_aux_assn\<^sup>k \<rightarrow>\<^sub>a sbi_aux_assn"
   unfolding signed_big_int_add_\<sigma>_eq_def
   by sepref
+
 sepref_def signed_big_int_add_\<sigma>_neq_impl is "uncurry signed_big_int_add_\<sigma>_neq"
   :: "sbi_aux_assn\<^sup>k *\<^sub>a sbi_aux_assn\<^sup>k \<rightarrow>\<^sub>a sbi_aux_assn"
   unfolding signed_big_int_add_\<sigma>_neq_def
   by sepref
 
-sepref_register "op_neq :: bool \<Rightarrow> _"
 sepref_def signed_big_int_add_impl is "uncurry signed_big_int_add"
   :: "sbi_aux_assn\<^sup>k *\<^sub>a sbi_aux_assn\<^sup>k \<rightarrow>\<^sub>a sbi_aux_assn"
   unfolding signed_big_int_add_def
   by sepref
+
 
 section "Subtraction"
 sepref_def signed_big_int_inv is "RETURN o signed_big_int_inv"
@@ -86,9 +118,52 @@ sepref_def signed_big_int_mult_school_impl is "uncurry signed_big_int_mult_schoo
   apply (rewrite al_fold_custom_empty[where 'l=size_t])
   apply (annot_snat_const size_t)
   by sepref
+    
+subsection \<open>Inversion\<close>
 
-(*
-export_llvm signed_big_int_mult_school_impl file "/tmp/mult.ll"
-*)
+sepref_def sbi_inv_impl is \<open>RETURN o sbi_inv\<close>
+  :: \<open>sbi_aux_assn\<^sup>d \<rightarrow>\<^sub>a sbi_aux_assn\<close>
+  unfolding sbi_inv_def
+  by sepref
+
+section \<open>Sepref Registrations\<close>
+text \<open>Now we register our implementations to refine HOL integers through @{term sbi_assn}\<close>
+
+sepref_register "0 :: int"
+sepref_register "1 :: int"
+
+context
+  notes [fcomp_norm_unfold] = sbi_assn_def[symmetric]
+begin
+
+lemmas signed_big_int_eq_impl_hnr[sepref_fr_rules] =
+  signed_big_int_eq_impl.refine[FCOMP signed_big_int_eq_refine]
+
+lemmas signed_big_int_neq_impl_hnr[sepref_fr_rules] =
+  signed_big_int_neq_impl.refine[FCOMP signed_big_int_neq_refine]
+
+lemmas signed_big_int0_impl_hnr[sepref_fr_rules] =
+  signed_big_int0_impl.refine[FCOMP signed_big_int0_refine]
+
+lemmas signed_big_int1_impl_hnr[sepref_fr_rules] =
+  signed_big_int1_impl.refine[FCOMP signed_big_int1_refine]
+
+lemmas signed_big_int_add_hnr[sepref_fr_rules] =
+  signed_big_int_add_impl.refine[FCOMP signed_big_int_add_refine]
+
+(* TODO: at some point this should probably be the more efficient Karatsuba implementation? *)
+lemmas signed_big_int_mult_school_hnr[sepref_fr_rules] =
+  signed_big_int_mult_school_impl.refine[FCOMP signed_big_int_mult_school_refine]
+
+lemmas sbi_inv_hnr[sepref_fr_rules] =
+  sbi_inv_impl.refine[FCOMP sbi_inv_ref]
+
+end
+
+text \<open>Deallocation of sbi temporaries (needed whenever a synthesis creates
+  intermediate sbi values, e.g. in \<open>n + m \<noteq> 0\<close>).\<close>
+schematic_goal sbi_assn_free[sepref_frame_free_rules]: "MK_FREE sbi_assn ?fr"
+  unfolding sbi_assn_def
+  by (rule MK_FREE_hrcompI mk_free_pair al_assn_free mk_free_pure mk_free_is_pure)+
 
 end
